Impredicativity

TT-model/semantics.lean
@@ -8,15 +8,20 @@ set_option pp.fieldNotation false
 
 variable [lc : LevelClass]
 
+-- Interpretation interface
+@[simp] def IInterp (a : Term) (P : Term → Prop) : Prop :=
+  ∃ (I : Term → (Term → Prop) → Prop),
+    I a P ∧ (∀ {a b}, a ⇒⋆ b → I b P → I a P)
+
+-- Interpretations of Type types
 inductive Interp (i : lc.L) (I : ∀ j, j < i → Term → Prop) : Term → (Term → Prop) → Prop where
   | pi a b Pa (Pf : Term → (Term → Prop) → Prop) :
     Interp i I a Pa →
     (∀ x, Pa x → ∃ Pb, Pf x Pb) →
     (∀ x Pb, Pf x Pb → Interp i I (subst (x +: var) b) Pb) →
     Interp i I (pi a b) (λ f ↦ ∀ x Pb, Pa x → Pf x Pb → Pb (app f x))
-  | 𝒰 j (lt : j < i) : Interp i I (𝒰 (lof j)) (I j lt)
-  | mty : Interp i I mty (λ _ ↦ False)
-  | lvl k : Interp i I (lvl (lof k)) (λ a ↦ ∃ j, a ⇒⋆ lof j ∧ j < k)
+  | 𝒰 j (lt : j < i) : Interp i I (𝒰 j) (I j lt)
+  | ℙ : Interp i I ℙ (∃ Pb, IInterp · Pb)
   | step a b P :
     a ⇒ b →
     Interp i I b P →
@@ -28,6 +33,17 @@ def Interps (i : lc.L) : Term → (Term → Prop) → Prop :=
 termination_by i
 
 notation:40 "⟦" a "⟧" i "↘" P => Interps i a P
+
+-- Interpretations of Prop types
+inductive Interp₀ : Term → (Term → Prop) → Prop where
+  | all i a b Pa (Pf : Term → (Term → Prop) → Prop) :
+    Interps i a Pa →
+    (∀ x, Pa x → ∃ Pb, Pf x Pb) →
+    (∀ x Pb, Pf x Pb → Interp₀ (subst (x +: var) b) Pb) →
+    Interp₀ (all a b) (λ f ↦ ∀ x Pb, Pa x → Pf x Pb → Pb (app f x))
+  | mty : Interp₀ mty (λ _ ↦ False)
+  | step a b P : a ⇒ b → Interp₀ b P → Interp₀ a P
+notation:40 "⟦" a "⟧ ↘" P => Interp₀ a P
 
 /-*------------------------
   Simple inversion lemmas
@@ -51,29 +67,50 @@ theorem interpPiInv {i I a b P} (h : ⟦ pi a b ⟧ i , I ↘ P) :
     . constructor <;> assumption
     . intro x Pb PfxPb; constructor <;> apply_rules [parCong, parRefl]
 
-theorem interp𝒰Inv {i I a P} (h : ⟦ 𝒰 a ⟧ i , I ↘ P) : ∃ j lt, a ⇒⋆ lof j ∧ P = I j lt := by
-  generalize e : 𝒰 a = b at h
-  induction h generalizing a <;> try contradiction
-  case 𝒰 j lt => injection e with e; subst e; exists j, lt, Pars.refl _
-  case step r _ ih =>
-    subst e; let (Par.𝒰 r₁) := r
-    let ⟨j, lt, r₂, e⟩ := ih rfl
-    exact ⟨j, lt, Pars.trans r₁ r₂, e⟩
+theorem interp𝒰Inv {i I j P} (h : ⟦ 𝒰 j ⟧ i , I ↘ P) : ∃ lt, P = I j lt := by
+  generalize e : 𝒰 j = b at h
+  induction h generalizing j <;> try contradiction
+  case 𝒰 j lt => injection e with e; subst e; exists lt
+  case step r _ ih => subst e; cases r; exact ih rfl
 
-theorem interpMtyInv {i I P} (h : ⟦ mty ⟧ i , I ↘ P) : P = (λ _ ↦ False) := by
+theorem interps𝒰Inv {i j P} (h : ⟦ 𝒰 j ⟧ i ↘ P) :
+  j < i ∧ P = λ a ↦ ∃ P, ⟦ a ⟧ j ↘ P := by
+  unfold Interps at h
+  let ⟨lt, e⟩ := interp𝒰Inv h
+  exact ⟨lt, e⟩
+
+theorem interpℙInv {i I P} (h : ⟦ ℙ ⟧ i , I ↘ P) : P = (∃ P, IInterp · P) := by
+  generalize e : ℙ = a at h
+  induction h <;> try contradiction
+  case ℙ => rfl
+  case step r _ ih => subst e; cases r; simp [ih]
+
+theorem interpsℙInv {i P} (h : ⟦ ℙ ⟧ i ↘ P) : P = (∃ P, IInterp · P) := by
+  unfold Interps at h; exact interpℙInv h
+
+theorem interpAllInv' {a b P} (h : ⟦ all a b ⟧ ↘ P) :
+  ∃ i Pa, ∃ (Pf : Term → (Term → Prop) → Prop),
+    (⟦ a ⟧ i ↘ Pa) ∧
+    (∀ x, Pa x → ∃ Pb, Pf x Pb) ∧
+    (∀ x Pb, Pf x Pb → Interp₀ (subst (x +: var) b) Pb) ∧
+    P = (λ f ↦ ∀ x Pb, Pa x → Pf x Pb → Pb (app f x)) := by
+  generalize e : all a b = c at h
+  induction h generalizing a b <;> try contradiction
+  case all Pa Pf ha hPf hb _ =>
+    injection e with ea eb; subst ea; subst eb
+    exact ⟨_, Pa, Pf, ha, hPf, hb, rfl⟩
+  case step r _ ih =>
+    subst e; cases r
+    let ⟨i, Pa, Pf, ha, hPf, hb, e⟩ := ih rfl
+    refine ⟨i, Pa, Pf, ?_, hPf, ?_, e⟩
+    . unfold Interps at *; constructor <;> assumption
+    . intro x Pb PfxPb; constructor <;> apply_rules [parCong, parRefl]
+
+theorem interpMtyInv {P} (h : ⟦ mty ⟧ ↘ P) : P = λ _ ↦ False := by
   generalize e : mty = a at h
   induction h <;> try contradiction
   case mty => rfl
   case step r _ ih => subst e; cases r; simp [ih]
-
-theorem interpLvlInv {i I a P} (h : ⟦ lvl a ⟧ i , I ↘ P) : ∃ k, a ⇒⋆ lof k ∧ P = (λ a ↦ ∃ j, a ⇒⋆ lof j ∧ j < k) := by
-  generalize e : lvl a = b at h
-  induction h generalizing a <;> try contradiction
-  case lvl k => injection e with e; subst e; exists k, Pars.refl _
-  case step r _ ih =>
-    subst e; let (Par.lvl r₁) := r
-    let ⟨k, r₂, e⟩ := ih rfl
-    exact ⟨k, Pars.trans r₁ r₂, e⟩
 
 /-*--------------------
   Better constructors
@@ -87,14 +124,18 @@ theorem interpsPi {i a b Pa P}
   unfold Interps at *; intro e; subst e; constructor; assumption; assumption; simp
 
 theorem interps𝒰 {i j} (lt : j < i) :
-  ⟦ 𝒰 (lof j) ⟧ i ↘ (λ a ↦ ∃ P, ⟦ a ⟧ j ↘ P) := by
+  ⟦ 𝒰 j ⟧ i ↘ (λ a ↦ ∃ P, ⟦ a ⟧ j ↘ P) := by
   unfold Interps at *; constructor; assumption
 
-theorem interpsMty {i} : ⟦ mty ⟧ i ↘ (λ _ ↦ False) := by
-  unfold Interps at *; constructor
+theorem interpsℙ {i} : ⟦ ℙ ⟧ i ↘ (∃ P, IInterp · P) := by
+  unfold Interps; constructor
 
-theorem interpsLvl {i k} : ⟦ lvl (lof k) ⟧ i ↘ (λ a ↦ ∃ j, a ⇒⋆ lof j ∧ j < k) := by
-  unfold Interps at *; constructor
+theorem interpsAll {i a b Pa P}
+  (ha : ⟦ a ⟧ i ↘ Pa)
+  (hb : ∀ x, Pa x → ∃ Pb, ⟦ subst (x +: var) b ⟧ ↘ Pb) :
+  P = (λ f ↦ ∀ x Pb, Pa x → (⟦ subst (x +: var) b⟧ ↘ Pb) → Pb (app f x)) →
+  ⟦ all a b ⟧ ↘ P := by
+  intro e; subst e; constructor; assumption; assumption; simp
 
 /-*------------------------------------------------
   Interpretation respects conversion wrt the type
@@ -105,9 +146,8 @@ theorem interpFwd {i I a b P} (r : a ⇒ b) (h : ⟦ a ⟧ i , I ↘ P) : ⟦ b 
   case pi iha ihb =>
     cases r; constructor
     all_goals intros; apply_rules [parCong, parRefl]
-  case 𝒰 => cases r; case 𝒰 r => cases r; constructor
-  case mty => cases r; constructor
-  case lvl => cases r; case lvl r => cases r; constructor
+  case 𝒰 => cases r; constructor
+  case ℙ => cases r; constructor
   case step r' _ ih =>
     let ⟨c, rc, rc'⟩ := diamond r r'
     constructor <;> apply_rules
@@ -115,18 +155,40 @@ theorem interpFwd {i I a b P} (r : a ⇒ b) (h : ⟦ a ⟧ i , I ↘ P) : ⟦ b 
 theorem interpsFwd {i a b P} (r : a ⇒ b) (h : ⟦ a ⟧ i ↘ P) : ⟦ b ⟧ i ↘ P := by
   unfold Interps at *; apply_rules [interpFwd]
 
-theorem interpsBwd {i a b P} (r : a ⇒ b) (h : ⟦ b ⟧ i ↘ P) : ⟦ a ⟧ i ↘ P := by
-  unfold Interps at *; constructor <;> assumption
+theorem interpFwd₀ {a b P} (r : a ⇒ b) (h : ⟦ a ⟧ ↘ P) : ⟦ b ⟧ ↘ P := by
+  induction h generalizing b
+  case all ihb =>
+    cases r; constructor
+    all_goals intros; apply_rules [interpsFwd, parCong, parRefl]
+  case mty => cases r; constructor
+  case step r' _ ih =>
+    let ⟨c, rc, rc'⟩ := diamond r r'
+    constructor <;> apply_rules
 
 theorem interpsFwds {i a b P} (r : a ⇒⋆ b) (h : ⟦ a ⟧ i ↘ P) : ⟦ b ⟧ i ↘ P := by
-  induction r generalizing P <;> apply_rules [interpsFwd]
+  induction r generalizing P
+  all_goals intros; apply_rules [interpsFwd]
+
+theorem interpFwds₀ {a b P} (r : a ⇒⋆ b) (h : ⟦ a ⟧ ↘ P) : ⟦ b ⟧ ↘ P := by
+  induction r generalizing P
+  all_goals intros; apply_rules [interpFwd₀]
+
+theorem interpsBwd {i a b P} (r : a ⇒ b) (h : ⟦ b ⟧ i ↘ P) : ⟦ a ⟧ i ↘ P := by
+  unfold Interps at *; constructor <;> assumption
 
 theorem interpsBwds {i a b P} (r : a ⇒⋆ b) (h : ⟦ b ⟧ i ↘ P) : ⟦ a ⟧ i ↘ P := by
   induction r generalizing P <;> apply_rules [interpsBwd]
 
+theorem interpBwds₀ {a b P} (r : a ⇒⋆ b) (h : ⟦ b ⟧ ↘ P) : ⟦ a ⟧ ↘ P := by
+  induction r generalizing P <;> apply_rules [Interp₀.step]
+
 theorem interpsConv {i a b P} (r : a ⇔ b) (h : ⟦ a ⟧ i ↘ P) : ⟦ b ⟧ i ↘ P :=
   let ⟨_, ra, rb⟩ := r
   interpsBwds rb (interpsFwds ra h)
+
+theorem interpConv₀ {a b P} (r : a ⇔ b) (h : ⟦ a ⟧ ↘ P) : ⟦ b ⟧ ↘ P :=
+  let ⟨_, ra, rb⟩ := r
+  interpBwds₀ rb (interpFwds₀ ra h)
 
 /-*----------------------------------------------------
   Backward preservation of interpretation predicate
@@ -139,11 +201,28 @@ theorem interpsBwdsP {i a x y P} (r : x ⇒⋆ y) (h : ⟦ a ⟧ i ↘ P) : P y 
     intro h x Pb Pax PfxPb
     exact ihb x Pb PfxPb (parsApp r (Pars.refl x)) (h x Pb Pax PfxPb)
   case 𝒰 => exact λ ⟨P, h⟩ ↦ ⟨P, interpsBwds r h⟩
-  case mty => simp
-  case lvl =>
-    intro ⟨j, r₂, lt⟩
-    exact ⟨j, parsTrans r r₂, lt⟩
+  case ℙ =>
+    intro ⟨P, I, hI, bwd⟩
+    exact ⟨P, I, bwd r hI, bwd⟩
   case step ih => exact ih r
+
+theorem interpBwdsP₀ {a x y P} (r : x ⇒⋆ y) (h : ⟦ a ⟧ ↘ P) : P y → P x := by
+  induction h generalizing x y
+  case all ihb =>
+    intro h x Pb Pax PfxPb
+    exact ihb x Pb PfxPb (parsApp r (Pars.refl x)) (h x Pb Pax PfxPb)
+  case mty => simp
+  case step ih => exact ih r
+
+/-*--------------------------------
+  Interpretations are propInterps
+--------------------------------*-/
+
+theorem interpsIInterp {i a P} (h : ⟦ a ⟧ i ↘ P) : IInterp a P :=
+  ⟨λ a P ↦ ⟦ a ⟧ i ↘ P, h, interpsBwds⟩
+
+theorem interpIInterp₀ {a P} (h : ⟦ a ⟧ ↘ P) : IInterp a P :=
+  ⟨λ a P ↦ ⟦ a ⟧ ↘ P, h, interpBwds₀⟩
 
 /-*--------------------------------
   Interpretation is deterministic
@@ -166,13 +245,8 @@ theorem interpDet' {i I a P Q} (hP : ⟦ a ⟧ i , I ↘ P) (hQ : ⟦ a ⟧ i , 
       let ⟨Pb', PfxPb'⟩ := hPf' x Pax'
       rw [ihb x Pb PfxPb (hb' x Pb' PfxPb')]
       exact h x Pb' Pax' PfxPb'
-  case 𝒰 =>
-    let ⟨j, _, r, e⟩ := interp𝒰Inv hQ
-    injection (parsLofInv r) with ej; subst ej; simp [e]
-  case mty => simp [interpMtyInv hQ]
-  case lvl =>
-    let ⟨k, r, e⟩ := interpLvlInv hQ
-    injection (parsLofInv r) with ek; subst ek; simp [e]
+  case 𝒰 => let ⟨_, e⟩ := interp𝒰Inv hQ; simp [e]
+  case ℙ => simp [interpℙInv hQ]
   case step r _ ih => exact ih (interpFwd r hQ)
 
 theorem interpsDet' {i a P Q} (hP : ⟦ a ⟧ i ↘ P) (hQ : ⟦ a ⟧ i ↘ Q) : P = Q := by
@@ -186,16 +260,35 @@ theorem interpsCumul {i j a P} (lt : i < j) (h : ⟦ a ⟧ i ↘ P) : ⟦ a ⟧ 
     . assumption
     . intro x Pb PfxPb; unfold Interps at ihb; exact ihb x Pb PfxPb lt
   case 𝒰 k _ => constructor; apply_rules [IsTrans.trans]
-  case mty => constructor
-  case lvl => constructor
+  case ℙ => constructor
   case step ih => constructor; assumption; unfold Interps at ih; exact ih lt
 
--- this is the only place we need trichotomy of <
+-- ⚠️ uses trichotomy of < ⚠️
 theorem interpsDet {i j a P Q} (hP : ⟦ a ⟧ i ↘ P) (hQ : ⟦ a ⟧ j ↘ Q) : P = Q := by
   rcases trichotomous (r := lc.lt.lt) i j with lt | eq | gt
   . exact interpsDet' (interpsCumul lt hP) hQ
   . rw [eq] at hP; apply interpsDet' hP hQ
   . exact interpsDet' hP (interpsCumul gt hQ)
+
+-- ⚠️ uses funext and propext ⚠️
+theorem interpDet₀ {a P Q} (hP : ⟦ a ⟧ ↘ P) (hQ : ⟦ a ⟧ ↘ Q) : P = Q := by
+  induction hP generalizing Q
+  case all Pa Pf ha hPf _ ihb =>
+    let ⟨i, Pa', Pf', ha', hPf', hb', e⟩ := interpAllInv' hQ
+    subst e; apply funext; intro f
+    apply propext; constructor
+    . intro h x Pb' Pax' PfxPb'
+      have Pax : Pa x := by rw [interpsDet ha ha']; exact Pax'
+      let ⟨Pb, PfxPb⟩ := hPf x Pax
+      rw [← ihb x Pb PfxPb (hb' x Pb' PfxPb')]
+      exact h x Pb Pax PfxPb
+    . intro h x Pb Pax PfxPb
+      have Pax' : Pa' x := by rw [interpsDet ha' ha]; exact Pax
+      let ⟨Pb', PfxPb'⟩ := hPf' x Pax'
+      rw [ihb x Pb PfxPb (hb' x Pb' PfxPb')]
+      exact h x Pb' Pax' PfxPb'
+  case mty => simp [interpMtyInv hQ]
+  case step r _ ih => exact ih (interpFwd₀ r hQ)
 
 /-*------------------------
   Better inversion lemmas
@@ -205,7 +298,7 @@ theorem interpsDet {i j a P Q} (hP : ⟦ a ⟧ i ↘ P) (hQ : ⟦ a ⟧ j ↘ Q)
 theorem interpPiInv' {i I a b P} (h : ⟦ pi a b ⟧ i , I ↘ P) :
   ∃ Pa, (⟦ a ⟧ i , I ↘ Pa) ∧
     (∀ x, Pa x → ∃ Pb, ⟦ subst (x +: var) b ⟧ i , I ↘ Pb) ∧
-    P = λ f ↦ ∀ x Pb, Pa x → (⟦ subst (x +: var) b⟧ i , I ↘ Pb) → Pb (app f x) := by
+    P = (λ f ↦ ∀ x Pb, Pa x → (⟦ subst (x +: var) b⟧ i , I ↘ Pb) → Pb (app f x)) := by
   let ⟨Pa, Pf, ha, hPf, hfb, e⟩ := interpPiInv h
   refine ⟨Pa, ha, ?_, ?_⟩
   . intro x Pax; let ⟨Pb, PfxPb⟩ := hPf x Pax
@@ -220,38 +313,74 @@ theorem interpPiInv' {i I a b P} (h : ⟦ pi a b ⟧ i , I ↘ P) :
 theorem interpsPiInv {i a b P} (h : ⟦ pi a b ⟧ i ↘ P) :
   ∃ Pa, (⟦ a ⟧ i ↘ Pa) ∧
     (∀ x, Pa x → ∃ Pb, ⟦ subst (x +: var) b ⟧ i ↘ Pb) ∧
-    P = λ f ↦ ∀ x Pb, Pa x → (⟦ subst (x +: var) b⟧ i ↘ Pb) → Pb (app f x) := by
+    P = (λ f ↦ ∀ x Pb, Pa x → (⟦ subst (x +: var) b⟧ i ↘ Pb) → Pb (app f x)) := by
   unfold Interps at *; exact interpPiInv' h
 
-theorem interps𝒰Inv {i a P} (h : ⟦ 𝒰 a ⟧ i ↘ P) :
-  ∃ j, j < i ∧ a ⇒⋆ lof j ∧ P = λ a ↦ ∃ P, ⟦ a ⟧ j ↘ P := by
-  unfold Interps at h
-  let ⟨j, lt, r, e⟩ := interp𝒰Inv h
-  exact ⟨j, lt, r, e⟩
-
-theorem interpsMtyInv {i P} (h : ⟦ mty ⟧ i ↘ P) : P = (λ _ ↦ False) := by
-  unfold Interps at h; exact interpMtyInv h
-
-theorem interpsLvlInv {i a P} (h : ⟦ lvl a ⟧ i ↘ P) : ∃ k, a ⇒⋆ lof k ∧ P = (λ a ↦ ∃ j, a ⇒⋆ lof j ∧ j < k) := by
-  unfold Interps at h; exact interpLvlInv h
+-- ⚠️ uses funext and propext ⚠️
+theorem interpAllInv {a b P} (h : ⟦ all a b ⟧ ↘ P) :
+  ∃ i Pa, (⟦ a ⟧ i ↘ Pa) ∧
+    (∀ x, Pa x → ∃ Pb, ⟦ subst (x +: var) b ⟧ ↘ Pb) ∧
+    P = (λ f ↦ ∀ x Pb, Pa x → (⟦ subst (x +: var) b⟧ ↘ Pb) → Pb (app f x)) := by
+  let ⟨i, Pa, Pf, ha, hPf, hfb, e⟩ := interpAllInv' h
+  refine ⟨i, Pa, ha, ?_, ?_⟩
+  . intro x Pax; let ⟨Pb, PfxPb⟩ := hPf x Pax
+    exact ⟨Pb, hfb x Pb PfxPb⟩
+  . subst e; apply funext; intro f; apply propext; constructor
+    . intro h x Pb Pax hb
+      let ⟨Pb', PfxPb'⟩ := hPf x Pax
+      have e : Pb = Pb' := by apply interpDet₀ hb (hfb x Pb' PfxPb')
+      rw [e]; apply_rules
+    . intros; apply_rules
 
 /-*----------------
   Semantic typing
 ----------------*-/
 
-def semSubst σ Γ := ∀ x a, In x a Γ → ∃ i P, (⟦ subst σ a ⟧ i ↘ P) ∧ P (σ x)
+open sort
+
+def semSubst σ Γ := ∀ x a,
+  (In 𝒰 x a Γ → ∃ i P, (⟦ subst σ a ⟧ i ↘ P) ∧ P (σ x)) ∧
+  (In ℙ x a Γ → ∃ P, (⟦ subst σ a ⟧ ↘ P) ∧ P (σ x))
 infix:40 "⊨" => semSubst
 
-def semWt Γ a A := ∀ σ, σ ⊨ Γ → ∃ i P, (⟦ subst σ A ⟧ i ↘ P) ∧ P (subst σ a)
-notation:40 Γ:41 "⊨" a:41 "∶" A:41 => semWt Γ a A
+def semWt𝒰 Γ a A := ∀ σ, σ ⊨ Γ → ∃ i P, (⟦ subst σ A ⟧ i ↘ P) ∧ P (subst σ a)
+notation:40 Γ:41 "⊨" a:41 "∶" A:41 => semWt𝒰 Γ a A
+
+def semWtℙ Γ a A := ∀ σ, σ ⊨ Γ → ∃ P, (⟦ subst σ A ⟧ ↘ P) ∧ P (subst σ a)
+notation:40 Γ:41 "⊨ₚ" a:41 "∶" A:41 => semWtℙ Γ a A
 
 theorem semSubstNil σ : σ ⊨ ⬝ := by
-  intro _ _ mem; cases mem
+  intros _ _; constructor
+  all_goals intro mem; cases mem
 
 theorem semSubstCons {Γ : Ctxt} {σ i a A P} :
   (⟦ subst σ A ⟧ i ↘ P) → P a →
   σ ⊨ Γ → a +: σ ⊨ Γ ∷ A := by
-  intro hA ha hσ x B mem
-  cases mem
-  case here => rw [substRenamed]; exists i, P
-  case there B mem => rw [substRenamed]; apply_rules [hσ]
+  intro hA ha hσ x B; constructor <;> intro mem
+  . cases mem
+    case here => rw [substRenamed]; exists i, P
+    case there x B mem =>
+      rw [substRenamed]
+      let ⟨in𝒰, _⟩ := hσ x B
+      exact in𝒰 mem
+  . cases mem
+    case there x B mem =>
+      rw [substRenamed]
+      let ⟨_, inℙ⟩ := hσ x B
+      exact inℙ mem
+
+theorem semSubstICons {Γ : Ctxt} {σ a A P} :
+  (⟦ subst σ A ⟧ ↘ P) → P a →
+  σ ⊨ Γ → a +: σ ⊨ Γ ∷ᵢ A := by
+  intro hA ha hσ x B; constructor <;> intro mem
+  . cases mem
+    case ithere x B mem =>
+      rw [substRenamed]
+      let ⟨in𝒰, _⟩ := hσ x B
+      exact in𝒰 mem
+  . cases mem
+    case ihere => rw [substRenamed]; exact ⟨P, hA, ha⟩
+    case ithere x B mem =>
+      rw [substRenamed]
+      let ⟨_, inℙ⟩ := hσ x B
+      exact inℙ mem
