TT-model/typing.lean
@@ -1,8 +1,10 @@
 import «TT-model».syntactics
 import «TT-model».reduction
 
-open Nat
+open Nat hiding all
 open Term
+open sort
+open LevelClass
 
 set_option autoImplicit false
 set_option pp.fieldNotation false
@@ -19,15 +21,16 @@ local infix:40 (priority := 1001) "≈" => Eqv -- override HasEquiv.Equiv
 
 inductive Eqv : Term → Term → Prop where
   | β {b a} : app (abs b) a ≈ subst (a +: var) b
-  | 𝒰 {a a'} :
-    a ≈ a' →
-    -----------
-    𝒰 a ≈ 𝒰 a'
   | pi {a a' b b'} :
     a ≈ a' →
     b ≈ b' →
     -----------------
     pi a b ≈ pi a' b'
+  | all {a a' b b'} :
+    a ≈ a' →
+    b ≈ b' →
+    -----------------
+    all a b ≈ all a' b'
   | abs {b b'} :
     b ≈ b' →
     --------------
@@ -41,10 +44,6 @@ inductive Eqv : Term → Term → Prop where
     b ≈ b' →
     --------------
     exf b ≈ exf b'
-  | lvl {a a'} :
-    a ≈ a' →
-    -----------
-    lvl a ≈ lvl a'
   | refl {a} : a ≈ a
   | sym {a b} :
     a ≈ b →
@@ -79,12 +78,11 @@ theorem convEqv {a b} : a ⇔ b → a ≈ b
 theorem eqvConv {a b} (r : a ≈ b) : a ⇔ b := by
   induction r
   case β => apply_rules [parConv, Par.β, parRefl]
-  case 𝒰 => apply_rules [conv𝒰]
   case pi => apply_rules [convPi]
+  case all => apply_rules [convAll]
   case abs => apply_rules [convAbs]
   case app => apply_rules [convApp]
   case exf => apply_rules [convExf]
-  case lvl => apply_rules [convLvl]
   case refl => apply convRefl
   case sym => apply_rules [convSym]
   case trans => apply_rules [convTrans]
@@ -105,9 +103,7 @@ theorem eqvConv {a b} (r : a ≈ b) : a ⇔ b := by
   will result in an ill-typed idx w.
 -------------------------------------------------*-/
 
-inductive I : Type where
-  | wf : I
-  | wt : I
+inductive I | wf | wt𝒰 | wtℙ
 open I
 
 structure T where
@@ -117,12 +113,14 @@ structure T where
 
 def idx : I → Type
   | wf => Ctxt
-  | wt => T
+  | wt𝒰 => T
+  | wtℙ => T
 
 section
 set_option hygiene false
 local notation:40 "⊢" Γ:40 => Wtf (Sigma.mk wf Γ)
-local notation:40 Γ:41 "⊢" a:41 "∶" A:41 => Wtf (Sigma.mk wt (T.mk Γ a A))
+local notation:40 Γ:41 "⊢" a:41 "∶" A:41 => Wtf (Sigma.mk wt𝒰 (T.mk Γ a A))
+local notation:40 Γ:41 "⊢ₚ" a:41 "∶" A:41 => Wtf (Sigma.mk wtℙ (T.mk Γ a A))
 
 inductive Wtf : (Σ w, idx w) → Prop where
   | nil : ⊢ ⬝
@@ -131,19 +129,29 @@ inductive Wtf : (Σ w, idx w) → Prop where
     Γ ⊢ A ∶ 𝒰 k →
     --------------
     ⊢ Γ ∷ A
+  | icons {Γ A} :
+    ⊢ Γ →
+    Γ ⊢ A ∶ ℙ →
+    --------------
+    ⊢ Γ ∷ A
   | var {Γ x A} :
     ⊢ Γ →
-    Γ ∋ x ∶ A →
-    -------------
+    Γ ∋ x ∶ A ∶ 𝒰 →
+    ----------------
     Γ ⊢ var x ∶ A
+  | ivar {Γ x A} :
+    ⊢ Γ →
+    Γ ∋ x ∶ A ∶ ℙ →
+    ---------------
+    Γ ⊢ₚ var x ∶ A
   | 𝒰 {Γ j k} :
-    Γ ⊢ j ∶ lvl k →
+    j < k →
     ---------------
     Γ ⊢ 𝒰 j ∶ 𝒰 k
   | pi {Γ A B k} :
     Γ ⊢ A ∶ 𝒰 k →
-    Γ ∷ A ⊢ B ∶ 𝒰 (rename succ k) →
-    --------------------------------
+    Γ ∷ A ⊢ B ∶ 𝒰 k →
+    ------------------
     Γ ⊢ pi A B ∶ 𝒰 k
   | abs {Γ A B b k} :
     Γ ⊢ pi A B ∶ 𝒰 k →
@@ -155,44 +163,64 @@ inductive Wtf : (Σ w, idx w) → Prop where
     Γ ⊢ a ∶ A →
     --------------------------------
     Γ ⊢ app b a ∶ subst (a +: var) B
-  | mty {Γ j k} :
-    Γ ⊢ j ∶ lvl k →
+  | ℙ {Γ} :
+    ⊢ Γ →
+    --------------
+    Γ ⊢ ℙ ∶ 𝒰 «0»
+  | all {Γ A B k} :
+    Γ ⊢ A ∶ 𝒰 k →
+    Γ ∷ A ⊢ B ∶ ℙ →
     ---------------
-    Γ ⊢ mty ∶ 𝒰 j
+    Γ ⊢ all A B ∶ ℙ
+  | iabs {Γ A B b k} :
+    Γ ⊢ A ∶ 𝒰 k →
+    Γ ∷ A ⊢ₚ b ∶ B →
+    --------------------
+    Γ ⊢ₚ abs b ∶ all A B
+  | iapp {Γ A B b a} :
+    Γ ⊢ₚ b ∶ all A B →
+    Γ ⊢ a ∶ A →
+    ---------------------------------
+    Γ ⊢ₚ app b a ∶ subst (a +: var) B
+  | mty {Γ} :
+    -----------
+    Γ ⊢ mty ∶ ℙ
   | exf {Γ A b k} :
     Γ ⊢ A ∶ 𝒰 k →
-    Γ ⊢ b ∶ mty →
-    -------------
+    Γ ⊢ₚ b ∶ mty →
+    --------------
     Γ ⊢ exf b ∶ A
-  | lvl {Γ a b k} :
-    Γ ⊢ a ∶ lvl b →
-    ----------------------
-    Γ ⊢ lvl a ∶ 𝒰 (lof k)
-  | lof {Γ j k} :
-    ⊢ Γ →
-    j < k →
-    -----------------------
-    Γ ⊢ lof j ∶ lvl (lof k)
-  | trans {Γ i j k} :
-    Γ ⊢ i ∶ lvl j →
-    Γ ⊢ j ∶ lvl k →
-    ---------------
-    Γ ⊢ i ∶ lvl k
+  | iexf {Γ A b} :
+    Γ ⊢ A ∶ ℙ →
+    Γ ⊢ₚ b ∶ mty →
+    --------------
+    Γ ⊢ₚ exf b ∶ A
   | conv {Γ A B a k} :
     A ≈ B →
     Γ ⊢ a ∶ A →
     Γ ⊢ B ∶ 𝒰 k →
     --------------
     Γ ⊢ a ∶ B
+  | iconv {Γ A B a} :
+    A ≈ B →
+    Γ ⊢ₚ a ∶ A →
+    Γ ⊢ B ∶ ℙ →
+    -----------
+    Γ ⊢ₚ a ∶ B
   | sub {Γ j k A} :
-    Γ ⊢ j ∶ lvl k →
+    j < k →
     Γ ⊢ A ∶ 𝒰 j →
-    ---------------
+    --------------
+    Γ ⊢ A ∶ 𝒰 k
+  | isub {Γ A k} :
+    Γ ⊢ A ∶ ℙ →
+    ------------
     Γ ⊢ A ∶ 𝒰 k
 end
 
 notation:40 "⊢" Γ:40 => Wtf (Sigma.mk wf Γ)
-notation:40 Γ:41 "⊢" a:41 "∶" A:41 => Wtf (Sigma.mk wt (T.mk Γ a A))
+notation:40 Γ:41 "⊢" a:41 "∶" A:41 => Wtf (Sigma.mk wt𝒰 (T.mk Γ a A))
+notation:40 Γ:41 "⊢ₚ" a:41 "∶" A:41 => Wtf (Sigma.mk wtℙ (T.mk Γ a A))
 
 theorem wtfApp {Γ A B B' b a}
   (hpi : Γ ⊢ b ∶ pi A B)
@@ -200,64 +228,3 @@ theorem wtfApp {Γ A B B' b a}
   (eB : B' = subst (a +: var) B) :
   Γ ⊢ app b a ∶ B' := by
   subst eB; constructor <;> assumption
-
-/-*---------------------------------------------
-  Lean currently doesn't support induction on
-  mutual inductives, nor structural recursion
-  on inductive predicates in Prop.
-  Put the below back when it does.
-
-mutual
-inductive Wf : Ctxt → Prop where
-  | nil : Wf nil
-  | cons {Γ A k} :
-    Wf Γ →
-    Wt Γ A (𝒰 k) →
-    ---------------
-    Wf (Γ ∷ A)
-
-inductive Wt : Ctxt → Term → Term → Prop where
-  | var {Γ x A} :
-    Wf Γ →
-    In x A Γ →
-    --------------
-    Wt Γ (var x) A
-  | 𝒰 {Γ j k} :
-    Wf Γ →
-    j < k →
-    Wt Γ (𝒰 j) (𝒰 k)
-  | pi {Γ A B k} :
-    Wt Γ A (𝒰 k) →
-    Wt (Γ ∷ A) B (𝒰 k) →
-    ---------------------
-    Wt Γ (pi A B) (𝒰 k)
-  | abs {Γ A B b k} :
-    Wt Γ (pi A B) (𝒰 k) →
-    Wt (Γ ∷ A) b B →
-    ----------------------
-    Wt Γ (abs b) (pi A B)
-  | app {Γ A B b a} :
-    Wt Γ b (pi A B) →
-    Wt Γ a A →
-    -----------------------------------
-    Wt Γ (app b a) (subst (a +: var) B)
-  | mty {Γ k} :
-    Wf Γ →
-    ---------------
-    Wt Γ mty (𝒰 k)
-  | exf {Γ A b k} :
-    Wt Γ A (𝒰 k) →
-    Wt Γ b mty →
-    --------------
-    Wt Γ (exf b) A
-  | conv {Γ A B a k} :
-    A ≈ B →
-    Wt Γ a A →
-    Wt Γ B (𝒰 k) →
-    ------------------
-    Wt Γ a B
-end
-
-prefix:95 "⊢" => Wf
-notation:40 Γ "⊢" a "∶" A => Wt Γ a A
----------------------------------------------*-/
