Main.lean
@@ -4,4 +4,3 @@ import «TT-model».reduction
 import «TT-model».typing
 import «TT-model».semantics
 import «TT-model».soundness
-import «TT-model».example
