TT-model/soundness.lean
@@ -4,127 +4,126 @@ import «TT-model».typing
 import «TT-model».semantics
 
 open Term
+open LevelClass
 
 set_option autoImplicit false
 set_option pp.fieldNotation false
 
-variable [lc : LevelClass]
+variable [LevelClass]
 
-theorem soundness {Γ a A} (h : Γ ⊢ a ∶ A) : Γ ⊨ a ∶ A := by
-  generalize e : @Sigma.mk I idx I.wt ⟨Γ, a, A⟩ = t at h
-  induction h generalizing Γ a A
-  all_goals injection e with eI e; injection eI
-  all_goals injection e with eCtxt eTerm eType;
-            subst eCtxt; subst eTerm; subst eType
+theorem soundness {idx} (h : Wtf idx) :
+  match idx with
+  | ⟨I.wt𝒰, ⟨Γ, a, A⟩⟩ => Γ ⊨ a ∶ A
+  | ⟨I.wtℙ, ⟨Γ, a, A⟩⟩ => Γ ⊨ₚ a ∶ A
+  | ⟨I.wf, _⟩ => True
+  := by
+  induction h
+  all_goals simp
   all_goals intro σ hσ
-  case var mem => apply hσ; assumption
+  case var x A _ mem _ => let ⟨in𝒰, _⟩ := hσ x A; exact in𝒰 mem
+  case ivar x A _ mem _ => let ⟨_, inℙ⟩ := hσ x A; exact inℙ mem
+  case 𝒰 j k ltj =>
+    let ⟨ℓ, ltk⟩ := exists_gt k
+    exact ⟨ℓ, _, interps𝒰 ltk, ⟨_, interps𝒰 ltj⟩⟩
   case pi ihA ihB =>
-    let ⟨i, P, h𝒰, hA⟩ := ihA rfl σ hσ
-    let ⟨_, _, ra, e⟩ := interps𝒰Inv h𝒰
+    simp [*] at *
+    let ⟨i, P, h𝒰, hA⟩ := ihA σ hσ
+    let ⟨_, e⟩ := interps𝒰Inv h𝒰
     exists i, P; subst e
     let ⟨PA, hA⟩ := hA
     constructor
     . assumption
     . constructor; apply interpsPi hA _ rfl
-      intro x PAx; rw [← substUnion]
-      let ⟨_, _, h𝒰, hB⟩ := ihB rfl (x +: σ) (semSubstCons hA PAx hσ)
-      let ⟨_, _, rb, e⟩ := interps𝒰Inv h𝒰
-      subst e; rw [substRenamed] at rb
-      let ⟨_, ra', rb'⟩ := confluence ra rb
-      rw [parsLofInv ra'] at rb'
-      injection (parsLofInv rb') with e
-      simp_rw [e, hB]
+      intro x PAx
+      change ∃ Pb, ⟦ subst (x +: var) (subst (⇑ σ) _) ⟧ _ ↘ Pb
+      rw [← substUnion]
+      let ⟨_, _, h𝒰, hB⟩ := ihB (x +: σ) (semSubstCons hA PAx hσ)
+      let ⟨_, e⟩ := interps𝒰Inv h𝒰
+      subst e; exact hB
   case abs ihpi ihb =>
-    let ⟨_, _, h𝒰, hpi⟩ := ihpi rfl σ hσ
-    let ⟨_, _, _, e⟩ := interps𝒰Inv h𝒰
+    let ⟨_, _, h𝒰, hpi⟩ := ihpi σ hσ
+    let ⟨_, e⟩ := interps𝒰Inv h𝒰
     subst e
     let ⟨P, hpi⟩ := hpi
     let ⟨Pa, hA, _, e⟩ := interpsPiInv hpi
     constructor; exists P; constructor
     . exact hpi
     . subst e; intro x Pb PAx hB; rw [← substUnion] at hB
-      let ⟨_, _, hB', hb⟩ := ihb rfl (x +: σ) (semSubstCons hA PAx hσ)
+      let ⟨_, _, hB', hb⟩ := ihb (x +: σ) (semSubstCons hA PAx hσ)
       rw [interpsDet hB hB']
-      apply interpsBwdsP _ hB' hb
-      apply parsβ
+      exact interpsBwdsP (parsβ _ _ _) hB' hb
   case app ihb iha =>
-    let ⟨i, _, hpi, hb⟩ := ihb rfl σ hσ
-    let ⟨_, PA, hA, ha⟩ := iha rfl σ hσ
+    let ⟨i, _, hpi, hb⟩ := ihb σ hσ
+    let ⟨_, PA, hA, ha⟩ := iha σ hσ
     let ⟨PA', hA', hB, e⟩ := interpsPiInv hpi
     rw [interpsDet hA hA'] at ha
     let ⟨PB, hB⟩ := hB (subst σ _) ha
     subst e; rw [← substDist]
     exists i, PB; constructor <;> apply_rules
-  case 𝒰 ih =>
-    let ⟨_, P, hk, hj⟩ := ih rfl σ hσ
-    let ⟨k, rk, e⟩ := interpsLvlInv hk
+  case ℙ =>
+    let ⟨«1», lt⟩ := exists_gt «0»
+    exists «1», (∃ P, ⟦ · ⟧ «0» ↘ P); constructor
+    . exact interps𝒰 lt
+    . constructor; exact interpsℙ
+  case all =>
+    exists «0», (∃ P, IInterp · P), interpsℙ
+    exists λ _ ↦ True, λ _ _ ↦ True; simp
+  case iabs ihA ihb =>
+    let ⟨_, _, h𝒰, hA⟩ := ihA σ hσ
+    let ⟨_, e⟩ := interps𝒰Inv h𝒰
     subst e
-    let ⟨j, rj, ltj⟩ := hj
-    let ⟨ℓ, ltk⟩ := exists_gt k
-    exists ℓ, (∃ P, ⟦ · ⟧ k ↘ P); constructor
-    . exact interpsBwds (pars𝒰 rk) (interps𝒰 ltk)
-    . constructor; exact interpsBwds (pars𝒰 rj) (interps𝒰 ltj)
-  case mty ih =>
-    let ⟨_, _, hj, hi⟩ := ih rfl σ hσ
-    let ⟨j, _, e⟩ := interpsLvlInv hj
-    subst e
-    let ⟨i, ri, lt⟩ := hi
-    refine ⟨j, (∃ P, ⟦ · ⟧ i ↘ P), ?_, ?_⟩
-    . exact interpsBwds (pars𝒰 ri) (interps𝒰 lt)
-    . constructor; exact interpsMty
-  case exf ihb _ _ =>
-    let ⟨_, _, hmty, hb⟩ := ihb rfl σ hσ
-    rw [interpsMtyInv hmty] at hb
+    let ⟨PA, hA⟩ := hA
+    constructor; constructor
+    . apply interpsAll hA ?_ rfl
+      intro x PAx
+      let ⟨PB, hB, _⟩ := ihb (x +: σ) (semSubstCons hA PAx hσ)
+      rw [substUnion] at hB; exists PB
+    . intro x PB PAx hB
+      let ⟨PB', hB', hb⟩ := ihb (x +: σ) (semSubstCons hA PAx hσ)
+      rw [← substUnion] at hB
+      rw [interpDet₀ hB hB']
+      exact interpBwdsP₀ (parsβ _ _ _) hB' hb
+  case iapp A _ _ _ _ _ ihb iha =>
+    let ⟨_, hall, hb⟩ := ihb σ hσ
+    let ⟨_, PA, hA, ha⟩ := iha σ hσ
+    let ⟨_, PA', hA', hB, e⟩ := interpAllInv hall
+    rw [interpsDet hA hA'] at ha
+    let ⟨PB, hB⟩ := hB (subst σ _) ha
+    subst e; rw [← substDist]
+    exists PB; constructor <;> apply_rules
+  case mty =>
+    refine ⟨«0», _, interpsℙ, ?_⟩
+    exists λ _ ↦ True, λ _ _ ↦ True; simp
+  case exf ihb =>
+    let ⟨_, hmty, hb⟩ := ihb σ hσ
+    rw [interpMtyInv hmty] at hb
     contradiction
-  case lvl k _ iha =>
-    let ⟨_, P, hlvl, ha⟩ := iha rfl σ hσ
-    let ⟨ℓ, lt⟩ := exists_gt k
-    refine ⟨ℓ, (∃ P, ⟦ · ⟧ k ↘ P), interps𝒰 lt, ?_⟩
-    let ⟨_, _, e⟩ := interpsLvlInv hlvl
-    subst e
-    let ⟨k, r, _⟩ := ha
-    exists (∃ j, · ⇒⋆ lof j ∧ j < k)
-    exact interpsBwds (parsLvl r) interpsLvl
-  case lof j k _ _ _ =>
-    refine ⟨j, (∃ j, · ⇒⋆ lof j ∧ j < k), interpsLvl, ?_⟩
-    exists j, Pars.refl _
-  case trans j k _ ihk _ ihj =>
-    let ⟨k, Pj, hk, hj⟩ := ihk rfl σ hσ
-    let ⟨k, _, ePj⟩ := interpsLvlInv hk
-    subst ePj
-    let ⟨j, rj, _⟩ := hj
-    let ⟨_, Pi, hj, hi⟩ := ihj rfl σ hσ
-    let ⟨j', rj', ePi⟩ := interpsLvlInv hj
-    subst ePi
-    let ⟨i, r, _⟩ := hi
-    let ⟨j'', rj, rj'⟩ := confluence rj rj'
-    rw [parsLofInv rj] at rj'
-    injection (parsLofInv rj') with e; subst e
-    refine ⟨_, (∃ j, · ⇒⋆ lof j ∧ j < k), hk, ?_⟩
-    exists i, r; apply IsTrans.trans <;> assumption
-  case conv iha conv _ _ =>
-    let ⟨i, P, hA, ha⟩ := iha rfl σ hσ
-    exists i, P; constructor
-    . exact interpsConv (convSubst σ (eqvConv conv)) hA
-    . exact ha
-  case sub ihj _ ihA =>
-    let ⟨_, Pj, h𝒰, hA⟩ := ihA rfl σ hσ
-    let ⟨j, _, rj, e⟩ := interps𝒰Inv h𝒰
+  case iexf ihb =>
+    let ⟨_, hmty, hb⟩ := ihb σ hσ
+    rw [interpMtyInv hmty] at hb
+    contradiction
+  case conv conv _ _ iha _ =>
+    let ⟨i, P, hA, ha⟩ := iha σ hσ
+    exact ⟨i, P, interpsConv (convSubst σ (eqvConv conv)) hA, ha⟩
+  case iconv conv _ _ iha _ =>
+    let ⟨P, hA, ha⟩ := iha σ hσ
+    exact ⟨P, interpConv₀ (convSubst σ (eqvConv conv)) hA, ha⟩
+  case sub j k _ ltj _ ihA =>
+    let ⟨_, Pj, h𝒰, hA⟩ := ihA σ hσ
+    let ⟨_, e⟩ := interps𝒰Inv h𝒰
     subst e
     let ⟨P, hA⟩ := hA
-    let ⟨_, Pk, hk, hj⟩ := ihj rfl σ hσ
-    let ⟨k, rk, e⟩ := interpsLvlInv hk
-    subst e
-    let ⟨j', rj', ltj'⟩ := hj
-    let ⟨j'', rj, rj'⟩ := confluence rj rj'
-    rw [parsLofInv rj'] at rj
-    injection (parsLofInv rj) with e; subst e
     let ⟨ℓ, ltk⟩ := exists_gt k
-    refine ⟨ℓ, (∃ P, ⟦ · ⟧ k ↘ P), ?_, ?_⟩
-    . exact interpsBwds (pars𝒰 rk) (interps𝒰 ltk)
-    . exists P; exact interpsCumul ltj' hA
+    exact ⟨ℓ, _, interps𝒰 ltk, ⟨P, interpsCumul ltj hA⟩⟩
+  case isub k _ ihA =>
+    let ⟨_, _, hℙ, hA⟩ := ihA σ hσ
+    rw [interpsℙInv hℙ] at hA
+    let ⟨P, hA⟩ := hA
+    let ⟨ℓ, ltk⟩ := exists_gt k
+    refine ⟨ℓ, _, interps𝒰 ltk, ⟨P, ?_⟩⟩
+    sorry
 
-theorem consistency {b} : ¬ ⬝ ⊢ b ∶ mty := by
+theorem consistency {b} : ¬ ⬝ ⊢ₚ b ∶ mty := by
   intro h
-  let ⟨_, _, hmty, hb⟩ := soundness h var (semSubstNil _)
-  simp [interpsMtyInv hmty] at hb
+  let ⟨_, hmty, hb⟩ := soundness h var (semSubstNil var)
+  simp [interpMtyInv hmty] at hb
